All builds.  Modify variable declaration to correctly put new name into scope before initialisation proceeds.  Also move towards correct handling of constructors, by having new sort of expression called the ConstructorFVal which sits in function position of a FnApp, and can be evaluated by expression evaluation.   Next steps: modify the VDecInit constructor to have two (rather more disjoint forms), with the second (corresponding to the current version with the argument of T) storing the address of the base of the object being initialised.  Multiple copies of this form will be created when an array is declared.   Also, complete rules for evaluation of arguments to constructors in meaning relation.   Finally, create one relation for handling as much of the variable declaration stuff as possible, thereby removing duplication between meaning and emeaning.

holsrcs/dynamicsScript.sml
@@ -1,4 +1,4 @@
-(* Dynamic Semantics of C(++) forms *)
+(* Dynamic Semantics of C++ forms *)
 
 (* Michael Norrish *)
 
@@ -321,7 +321,7 @@ val signed_int_def = Define`
 
 (* note that this predicate is two-valued: the possibility that a value
    isn't well-defined for the type is ignored.  This is because we assume
-   that possibility is dealt with elsewher: when values are read out of
+   that possibility is dealt with elsewhere: when values are read out of
    memory or otherwise constructed. *)
 val is_zero_def = Define`
   (is_zero (Signed i) v = (INT_VAL (Signed i) v = SOME 0)) /\
@@ -343,27 +343,30 @@ val final_value_def = Define`
 `;
 
 val vdeclare_def = Define`
-  vdeclare s0 ty nm optval s =
-     (?a sz s' rs.
+  vdeclare s0 ty nm s =
+     (?a sz rs.
          (rs = range_set a sz) /\
          object_type ty /\ malloc s0 ty a /\ sizeof (sizeofmap s) ty sz /\
-         (s' = s0 with <| allocmap updated_by (UNION) rs;
-                           varmap updated_by
-                              (\vm. vm |+ (nm,(a,default_path ty)));
-                           typemap updated_by (\tm. tm |+ (nm,ty)) |>) /\
-         (case optval of
-             NONE -> (s = s')
-          || SOME (ECompVal v ty') ->
-                (s = val2mem (s' with initmap updated_by (UNION) rs) a v)
-          || SOME other -> F))
+         (s = s0 with <| allocmap updated_by (UNION) rs;
+                          varmap updated_by
+                             (\vm. vm |+ (nm,(a,default_path ty)));
+                          typemap updated_by (\tm. tm |+ (nm,ty)) |>))
         \/
      (function_type ty /\
       (s = s0 with typemap updated_by (\tm. tm |+ (nm, ty))))
         \/
-     (?a t ty0 p.
-        (ty = Ref ty0) /\ (optval = SOME (LVal a t p)) /\
-        (s = s0 with <| varmap updated_by (\vm. vm |+ (nm, (a, p)));
-                        typemap updated_by (\tm. tm |+ (nm, ty)) |>))
+     (?ty0.
+        (ty = Ref ty0) /\
+        (* before the reference gets initialised, what should its value be?
+           Or, what does an uninitialised reference what look like?
+           Certainly, references must be initialised by valid objects, so
+           attempting
+              int &y = y ;
+           must be bad.  So, let's make it a reference to a guaranteed bad
+           address, 0 *)
+        (s = s0 with
+             <| varmap updated_by (\vm. vm |+ (nm, (0, default_path ty0)));
+                typemap updated_by (\tm. tm |+ (nm, ty0)) |>))
 
 `;
 
@@ -374,6 +377,7 @@ val copy2globals_def = Define`
 `;
 
 (* true if the nth argument of f is not a reference type *)
+(* TODO: deal with overloading *)
 val fn_expects_rval_def = Define`
   fn_expects_rval s f n =
     ?retty args.
@@ -381,6 +385,15 @@ val fn_expects_rval_def = Define`
        expr_type (expr_type_comps s) RValue f (Ptr (Function retty args))) /\
       ~ref_type (EL n args)
 `;
+
+(* true if the nth argument of the constructor for cnm is not a reference
+   type - the actual arguments are passed so that we have a hope of figuring
+   out which actual constructor is going to get called *)
+(* TODO: deal with overloading *)
+(* TODO: complete definition of constructor_expects_rval *)
+val constructor_expects_rval_def = Define`
+  constructor_expects_rval s cnm arglist n = T
+`
 
 val return_cont_def = Define`
   return_cont ty = if ref_type ty then LVC LVal
@@ -660,6 +673,7 @@ val (meaning_rules, meaning_ind, meaning_cases) = Hol_reln`
 
    /\
 
+(* RULE-ID: deref-objptr *)
 (* 5.3.1 p1 - pointer to an object type *)
 (!mval t se s addr pth.
      object_type t /\ (SOME (addr,pth) = ptr_decode(s,t) mval)
@@ -669,6 +683,7 @@ val (meaning_rules, meaning_ind, meaning_cases) = Hol_reln`
 
    /\
 
+(* RULE-ID: deref-objptr-fails *)
 (!mval t se s.
      object_type t /\ (ptr_decode(s,t) mval = NONE)
    ==>
@@ -677,6 +692,7 @@ val (meaning_rules, meaning_ind, meaning_cases) = Hol_reln`
 
    /\
 
+(* RULE-ID: deref-fnptr *)
 (* 5.3.1 p1 - pointer to a function type *)
 (!v retty argtys se s.
      v IN FDOM s.fndecode
@@ -810,6 +826,20 @@ val (meaning_rules, meaning_ind, meaning_cases) = Hol_reln`
    ==>
      ^mng (mExpr (FnApp (FVal fnid fty eopt) params) se) s
           (s, ev (FnApp_sqpt (FVal fnid fty eopt) params) base_se))
+
+   /\
+
+(* RULE-ID: constructor-call-sqpt *)
+(!cnm params se s.
+     EVERYi (\i e. if constructor_expects_rval s cnm params i then
+                     ?a t p. e = LVal a t p
+                   else
+                     ?v t. e = ECompVal v t)
+            params /\
+     is_null_se se
+   ==>
+     ^mng (mExpr (FnApp (ConstructorFVal cnm) params) se) s
+          (s, ev (FnApp_sqpt (ConstructorFVal cnm) params) base_se))
 
    /\
 
@@ -1073,50 +1103,108 @@ val (meaning_rules, meaning_ind, meaning_cases) = Hol_reln`
 
    /\
 
-(* RULE-ID: block-vdec *)
+(* RULE-ID: block-vdec-nonclass *)
 (!s0 s ty name vds sts c.
-     vdeclare s0 ty name NONE s
+     vdeclare s0 ty name s /\ (!cnm. ~(ty = Class cnm))
    ==>
      ^mng (mStmt (Block T (VDec ty name :: vds) sts) c) s0
           (s, mStmt (Block T vds sts) c))
 
    /\
 
-(* RULE-ID: block-vdecinit-evaluate *)
-(!ty name exte exte' s0 s vds sts c.
-     ^mng exte s0 (s, exte')
+(* RULE-ID: block-vdec-class *)
+(* if called on to declare a class variable, then the default, argument-less
+   constructor gets called *)
+(* TODO: handle construction of arrays of objects, which happens in order
+   of increasing subscripts (see 12.6 p3) *)
+(!s0 s name cnm vds sts c.
+     vdeclare s0 (Class cnm) name s
    ==>
-     ^mng (mStmt (Block T (VDecInit ty name exte::vds) sts) c) s0
-          (s, mStmt (Block T (VDecInit ty name exte'::vds) sts) c))
+     ^mng (mStmt (Block T (VDec (Class cnm) name :: vds) sts) c) s0
+          (s, mStmt (Block
+                       T
+                       (CONS (VDecInit
+                                (Class cnm)
+                                name
+                                T
+                                (DirectInit
+                                   (NormE (FnApp
+                                             (ConstructorFVal cnm)
+                                             [])
+                                          base_se)))
+                             vds)
+                       sts)
+                    c))
+
+   /\
+
+(* RULE-ID: block-vdecinit-start-evaluate *)
+(* internal flag switches from F to T *)
+(!ty name ii s0 s vds sts c.
+     vdeclare s0 ty name s
+   ==>
+     ^mng (mStmt (Block T (VDecInit ty name F ii::vds) sts) c) s0
+          (s, mStmt (Block T (VDecInit ty name T ii::vds) sts) c))
+
+   /\
+
+(* RULE-ID: block-vdecinit-evaluate *)
+(!ty name exte0 exte s0 s vds sts c f.
+     ^mng exte0 s0 (s, exte) /\ ((f = CopyInit) \/ (f = DirectInit))
+   ==>
+     ^mng (mStmt (Block T (VDecInit ty name T (f exte0) :: vds) sts) c) s0
+          (s, mStmt (Block T (VDecInit ty name T (f exte) :: vds) sts) c))
 
    /\
 
 (* RULE-ID: block-vdecinit-lval2rval *)
-(!s0 e0 se0 s e se ty name vds sts c.
-     lval2rval (s0,e0,se0) (s,e,se) /\ ~ref_type ty
+(!s0 e0 se0 s e se ty name vds sts c f.
+     lval2rval (s0,e0,se0) (s,e,se) /\ ~ref_type ty /\
+     ((f = CopyInit) \/ (f = DirectInit))
    ==>
-     ^mng (mStmt (Block T (VDecInit ty name (mExpr e0 se0) :: vds) sts) c) s0
-          (s, mStmt (Block T (VDecInit ty name (mExpr e se) :: vds) sts) c))
+     ^mng (mStmt (Block T
+                        (VDecInit ty name T (f (mExpr e0 se0)) :: vds)
+                        sts)
+                 c) s0
+          (s, mStmt (Block T
+                           (VDecInit ty name T (f (mExpr e se)) :: vds)
+                           sts)
+                    c))
 
    /\
 
-(* RULE-ID: block-vdecinit-finish-nonref *)
-(!dty name v ty v' se vds sts c s0 s.
-     is_null_se se /\ vdeclare s0 dty name (SOME (ECompVal v' dty)) s /\
-     parameter_coerce (v,ty) (v',dty)
+(* RULE-ID: block-vdecinit-finish *)
+(* for non-class, non-reference declarations.  Non-class is checked for
+   explicitly.  Non-reference is implicit in that the RHS has evaluated as
+   far as an ECompVal *)
+(!dty name v ty v' se vds sts c s0 s rs f a pth.
+     is_null_se se /\
+     (!cnm. ~(dty = Class cnm)) /\
+     ((a,pth) = s0.varmap ' name) /\
+     parameter_coerce (v,ty) (v',dty) /\
+     (rs = range_set a (LENGTH v')) /\
+     (s = val2mem (s0 with initmap updated_by (UNION) rs) a v') /\
+     ((f = CopyInit) \/ (f = DirectInit))
    ==>
-     ^mng (mStmt (Block T (VDecInit dty name (NormE (ECompVal v ty) se) :: vds)
-                          sts) c)
+     ^mng (mStmt (Block T
+                        (VDecInit dty name T
+                                  (f (NormE (ECompVal v ty) se)) :: vds)
+                        sts) c)
           s0
           (s, mStmt (Block T vds sts) c))
 
    /\
 
 (* RULE-ID: block-vdecinit-finish-ref *)
-(!se s0 ty name a t p s vds sts c.
-     is_null_se se /\ vdeclare s0 ty name (SOME (LVal a t p)) s
+(!se s0 ty1 ty2 name a p s vds sts c f.
+     is_null_se se /\ ((f = CopyInit) \/ (f = DirectInit)) /\
+     (s = s0 with varmap updated_by (\fm. fm |+ (name, (a,p))))
    ==>
-     ^mng (mStmt (Block T (VDecInit ty name (NormE (LVal a t p) se) :: vds)
+     ^mng (mStmt (Block T (VDecInit
+                             (Ref ty1)
+                             name
+                             T
+                             (f (NormE (LVal a ty2 p) se)) :: vds)
                         sts) c)
           s0
           (s, mStmt (Block T vds sts) c))
@@ -1184,50 +1272,97 @@ val (emeaning_rules, emeaning_ind, emeaning_cases) = Hol_reln`
 
    /\
 
-(* RULE-ID: global-var-defn *)
+(* RULE-ID: global-nonclass-var-defn *)
 (!s0 ty name s edecls.
-     vdeclare s0 ty name NONE s /\ object_type ty
+     vdeclare s0 ty name s /\ object_type ty /\ (!cnm. ~(ty = Class cnm))
    ==>
-     emeaning (Decl (VDec ty name) :: edecls) s0 (copy2globals s, edecls)) /\
+     emeaning (Decl (VDec ty name) :: edecls) s0 (copy2globals s, edecls))
+
+   /\
+
+(* RULE-ID: global-class-var-defn *)
+(!s0 cnm name s edecls.
+     vdeclare s0 (Class cnm) name s
+   ==>
+     emeaning (Decl (VDec (Class cnm) name) :: edecls)
+              s0
+              (copy2globals s,
+               CONS (Decl
+                       (VDecInit (Class cnm)
+                                 name
+                                 T
+                                 (DirectInit
+                                    (NormE (FnApp
+                                              (ConstructorFVal cnm)
+                                              [])
+                                           base_se))))
+                    edecls))
+
+   /\
+
+(* RULE-ID: global-vdecinit-start-evaluate *)
+(* internal flag switches from F to T *)
+(!s0 ty name ii edecls s.
+     vdeclare s0 ty name s
+   ==>
+     emeaning (Decl (VDecInit ty name F ii) :: edecls) s0
+              (s, Decl (VDecInit ty name T ii) :: edecls))
+
+   /\
+
 
 (* RULE-ID: global-var-init-evaluation *)
-(!s0 ty name exte exte' edecls s.
-     meaning exte s0 (s, exte')
+(!s0 ty name exte exte' edecls s f.
+     meaning exte s0 (s, exte') /\
+     ((f = CopyInit) \/ (f = DirectInit))
    ==>
-     emeaning (Decl (VDecInit ty name exte) :: edecls) s0
-              (s, Decl (VDecInit ty name exte') :: edecls))
+     emeaning (Decl (VDecInit ty name T (f exte)) :: edecls) s0
+              (s, Decl (VDecInit ty name T (f exte')) :: edecls))
 
    /\
 
 (* RULE-ID: global-var-init-lval2rval *)
-(!ty name e0 se0 edecls s0 s e se.
-     lval2rval (s0,e0,se0) (s,e,se) /\ ~ref_type ty
+(!ty name e0 se0 edecls s0 s e se f.
+     lval2rval (s0,e0,se0) (s,e,se) /\ ~ref_type ty /\
+     ((f = CopyInit) \/ (f = DirectInit))
    ==>
-     emeaning (Decl (VDecInit ty name (mExpr e0 se0)) :: edecls) s0
-              (s, Decl (VDecInit ty name (mExpr e se)) :: edecls))
+     emeaning (Decl (VDecInit ty name T (f (mExpr e0 se0))) :: edecls) s0
+              (s, Decl (VDecInit ty name T (f (mExpr e se))) :: edecls))
 
    /\
 
-(* RULE-ID: global-var-init-eval-finished *)
-(!s0 s name v ty dty v' edecls se.
-     vdeclare s0 dty name (SOME (ECompVal v' dty)) s /\
+(* RULE-ID: global-vdecinit-finish *)
+(* analogue of block-vdecinit-finish *)
+(* TODO: merge this with one indepedent vdec relation *)
+(!s0 s name v ty dty v' edecls se a pth rs f.
      parameter_coerce (v,ty) (v',dty) /\
-     is_null_se se /\ ~ref_type dty
+     is_null_se se /\
+     (!cnm. ~(dty = Class cnm)) /\
+     ((a,pth) = s0.varmap ' name) /\
+     (s = val2mem (s0 with initmap updated_by (UNION) rs) a v') /\
+     (rs = range_set a (LENGTH v')) /\
+     ((f = CopyInit) \/ (f = DirectInit))
    ==>
-     emeaning (Decl (VDecInit dty name (NormE (ECompVal v ty) se)) :: edecls)
-              s0
-              (copy2globals s, edecls))
+     emeaning
+       (Decl (VDecInit dty name T (f (NormE (ECompVal v ty) se))) :: edecls)
+       s0
+       (copy2globals s, edecls))
 
    /\
 
-(* RULE-ID: global-var-init-eval-ref-finished *)
-(!s0 ty name a t p s se edecls.
-     vdeclare s0 ty name (SOME (LVal a t p)) s /\ is_null_se se /\
-     ref_type ty
+(* RULE-ID: global-vdecinit-finish-ref *)
+(* analogue of block-vdecinit-finish-ref *)
+(* TODO: merge with independent vdec relation *)
+(!s0 ty1 name a ty2 p s se edecls f.
+     is_null_se se /\ ((f = CopyInit) \/ (f = DirectInit)) /\
+     (s = s0 with varmap updated_by (\fm. fm |+ (name, (a, p))))
    ==>
-     emeaning (Decl (VDecInit ty name (NormE (LVal a t p) se)) :: edecls)
-              s0
-              (copy2globals s, edecls))
+     emeaning
+       (CONS
+          (Decl (VDecInit (Ref ty1) name T (f (NormE (LVal a ty2 p) se))))
+          edecls)
+       s0
+       (copy2globals s, edecls))
 
    /\
 
